extract/Extract.v
@@ -1,0 +1,5 @@
+Require Import Ssara.Base.Vm.
+
+Require Extraction.
+Extraction Language OCaml.
+Extraction "run.ml" run.
