Makefile
@@ -1,0 +1,14 @@
+all: base extract
+
+base:
+	+make -C base
+.PHONY: base
+
+extract:
+	+make -C extract
+.PHONY: base
+
+clean:
+	+make -C base clean
+	+make -C extract clean
+.PHONY: clean
