build_makefile.sh
@@ -1,5 +1,0 @@
-#!/usr/bin/sh
-
-set -xe
-
-coq_makefile -f _CoqProject -o Makefile
